code/tests/Hacl.Test.Circuits.fst
@@ -1,0 +1,42 @@
+module Hacl.Test.Circuits
+
+open Lib.Sliceable
+open Lib.Circuits
+open FStar.Tactics
+
+module UI=FStar.UInt
+
+let m:pos = 1
+let p:pos = 4
+
+let circ : circuit m p =
+  let rec aux (i:nat) : circuit m (i+1) =
+    if i=0 then
+      Cons Empty (Input 0)
+    else
+      Cons (aux (i-1)) (Xor (i-1) (i-1))
+  in
+  aux (p-1)
+
+let impl (lN:bar) (x:xNxM lN.xN m) : xNxM lN.xN p =
+  circuit_spec2 circ lN x
+
+let spec (a:UI.uint_t m) : UI.uint_t p = a % 2
+
+let foo (lN:bar) : Lemma (
+  forall (x:xNxM lN.xN m) (j:nat{j<lN.xN.n}).
+  column j (impl lN x) == of_uint (spec (to_uint (column j x)))
+  ) =
+  let impl' (x:x1xM bool m) : x1xM bool p = impl l1 x in
+  circuit_spec2_sliceable circ lN;
+  assert(sliceable (impl lN) impl');
+  assert(let i = 1 in x1xM_eq (impl' (of_uint i)) (of_uint (spec i))) by (
+    //norm [ delta_only [`%impl; `%l1; `%x1; `%Mkfoo?.t]; delta; iota; primops; simplify; nbe ];
+    norm [ delta; iota; primops; simplify; nbe ];
+    norm [ zeta; delta_only [`%circuit_spec2] ];
+    norm [ delta; iota; primops; simplify; nbe ];
+    dump "";
+    //norm [ delta; zeta; iota; primops; simplify; nbe ];
+    qed ()
+  );
+  admit ()
